% !TeX root = ../../main.tex
\documentclass[../methodology.tex]{subfiles}
\begin{document}
\subsection{Geometric properties}
\subsubsection{Embedding}
\begin{definition}\label{M:Embedding}
  Let \(N=\left(P,g\right)\) be a \(n\)-dimension Riemannian manifold
  on position parameter space with such inner product \(g\) that
  the map \(f={\psi_0}^{-1}\)
  is an isometric embedding to \(\left(n+1\right)\)-manifold
  with the metric of \(g=\diag{\left(\sign{\lambda},1,\dots,1\right)}\).
\end{definition}
\begin{lemma}\label{M:Tangent:Basis}
  Position parameter \(\tensor{\theta}{^i}\) is associated to the following vector in position (tangent) vector space.
  \[
    \frac{\partial}{\partial\tensor{\theta}{^i}}=
    \begin{pmatrix}
      -\lambda\tan_\lambda^\ast\tensor{\theta}{^i}\tensor{p}{^j}         \\
      \lambda\frac{1}{\tan_\lambda\tensor{\theta}{^i}}\tensor{p}{^{i+1}} \\
      0
    \end{pmatrix}\frac{\partial}{\partial\tensor{p}{^j}}
  \]
\end{lemma}
\begin{proof}[Proof of \cref{M:Tangent:Basis}]
  \begin{align*}
    \frac{\partial}{\partial\tensor{\theta}{^i}}
     & =\frac{\partial\tensor{p}{^j}}{\partial\tensor{\theta}{^i}}\frac{\partial}{\partial\tensor{p}{^j}}                                                                        \\
     & =\frac{\partial}{\partial\tensor{\theta}{^i}}
    \left[
      \frac{1}{\lambda}
      \begin{pmatrix}
        \prod_{l\in\Set{1..n}}{\cos_\lambda{\tensor{\theta}{^l}}}                                      \\
        \sin_\lambda{\tensor{\theta}{^{j-1}}}\prod_{l\in\Set{j..n}}{\cos_\lambda{\tensor{\theta}{^l}}} \\
        \sin_\lambda{{\tensor{\theta}{^n}}}                                                            \\
      \end{pmatrix}
    \right]\frac{\partial}{\partial\tensor{p}{^j}}                                                                                                                               \\
     & =
    \frac{1}{\lambda}
    \frac{\partial}{\partial\tensor{\theta}{^i}}
    \left[
      \begin{pmatrix}
        \prod_{l\in\Set{1..n}}{\cos_\lambda{\tensor{\theta}{^l}}}                                      \\
        \sin_\lambda{\tensor{\theta}{^{j-1}}}\prod_{l\in\Set{j..n}}{\cos_\lambda{\tensor{\theta}{^l}}} \\
        \sin_\lambda{{\tensor{\theta}{^n}}}                                                            \\
      \end{pmatrix}
    \right]\frac{\partial}{\partial\tensor{p}{^j}}                                                                                                                               \\
     & =
    \frac{1}{\lambda}
    \begin{pmatrix}
      -\lambda\sin_\lambda^\ast{\tensor{\theta}{^i}}\prod_{l\in\Set{1..n}/\Set{i}}{\cos_\lambda{\tensor{\theta}{^l}}}                                      \\
      -\lambda\sin_\lambda^\ast{\tensor{\theta}{^i}}\sin_\lambda{\tensor{\theta}{^{j-1}}}\prod_{l\in\Set{j..n}/\Set{i}}{\cos_\lambda{\tensor{\theta}{^l}}} \\
      \lambda\cos_\lambda{\tensor{\theta}{^{i}}}\prod_{l\in\Set{i+1..n}}{\cos_\lambda{\tensor{\theta}{^l}}}                                                \\
      0                                                                                                                                                    \\
    \end{pmatrix}\frac{\partial}{\partial\tensor{p}{^j}} \\
     & =
    \begin{pmatrix}
      -\tan_\lambda^\ast{\tensor{\theta}{^i}}\prod_{l\in\Set{1..n}}{\cos_\lambda{\tensor{\theta}{^l}}}                                      \\
      -\tan_\lambda^\ast{\tensor{\theta}{^i}}\sin_\lambda{\tensor{\theta}{^{j-1}}}\prod_{l\in\Set{j..n}}{\cos_\lambda{\tensor{\theta}{^l}}} \\
      \frac{1}{\tan_\lambda{\tensor{\theta}{^{i}}}}\prod_{l\in\Set{i+1..n}}{\cos_\lambda{\tensor{\theta}{^l}}}                              \\
      0                                                                                                                                     \\
    \end{pmatrix}
    \frac{\partial}{\partial\tensor{p}{^j}}                                                                                                                                      \\
     & =
    \lambda
    \begin{pmatrix}
      -\tan_\lambda^\ast\tensor{\theta}{^i}\tensor{p}{^j}         \\
      \frac{1}{\tan_\lambda\tensor{\theta}{^i}}\tensor{p}{^{i+1}} \\
      0
    \end{pmatrix}\frac{\partial}{\partial\tensor{p}{^j}}
     & \qedhere
  \end{align*}
\end{proof}
\begin{lemma}\label{M:MetricTensor}
  The metric tensor of \(N\) at \(P\equiv\tensor{\theta}{}\) is
  \[
    \tensor{g}{_a_b}=
    \begin{cases}
      \prod_{a<j}{\cos_\lambda^2\tensor{\theta}{^j}} & \text{if \(a=b\),} \\
      0                                              & \text{otherwise.}  \\
    \end{cases}
  \]
\end{lemma}
\begin{proof}[Proof of \cref{M:MetricTensor}]
  \begin{align*}
    \tensor{g}{_a_b}\left[\frac{\partial}{\partial\tensor{\theta}{^i}}\right]
     & =\sum_{l,m=1}^{n+1}{
    \frac{\partial{\tensor{p}{^l}}}{\partial{\tensor{\theta}{^a}}}
    \tensor{g}{_l_m}\left[\frac{\partial}{\partial\tensor{p}{^i}}\right]
    \frac{\partial{\tensor{p}{^m}}}{\partial{\tensor{\theta}{^b}}}
    }                       \\
     & =
    \left(\sign{\lambda}\right)
    \frac{\partial{\tensor{p}{^1}}}{\partial{\tensor{\theta}{^a}}}
    \frac{\partial{\tensor{p}{^1}}}{\partial{\tensor{\theta}{^b}}}
    +
    \sum_{l=2}^{n+1}{
    \frac{\partial{\tensor{p}{^l}}}{\partial{\tensor{\theta}{^a}}}
    \frac{\partial{\tensor{p}{^l}}}{\partial{\tensor{\theta}{^b}}}
    }
  \end{align*}
  If \(a<b\),
  \begin{align*}
    \tensor{g}{_a_b}
     & =\left(
    \lambda
    \begin{pmatrix}
        -\tan_\lambda^\ast\left(\tensor{\theta}{^a}\right)\tensor{p}{^j}         \\
        \frac{1}{\tan_\lambda\left(\tensor{\theta}{^a}\right)}\tensor{p}{^{a+1}} \\
        0                                                                        \\
      \end{pmatrix}\right)
    \tensor{g}{}\left[\frac{\partial}{\partial\tensor{p}{^i}}\right]
    \left(
    \lambda
    \begin{pmatrix}
        -\tan_\lambda^\ast\left(\tensor{\theta}{^b}\right)\tensor{p}{^j}         \\
        \frac{1}{\tan_\lambda\left(\tensor{\theta}{^b}\right)}\tensor{p}{^{b+1}} \\
        0                                                                        \\
      \end{pmatrix}\right) \\
     & =
    \lambda^2
    \left(
    \left(\sign{\lambda}\right)\tan_\lambda^\ast\left(\tensor{\theta}{^a}\right)\tan_\lambda^\ast\left(\tensor{\theta}{^b}\right){\tensor{p}{^1}}^2
    +
    \sum_j{\tan_\lambda^\ast\left(\tensor{\theta}{^a}\right)\tan_\lambda^\ast\left(\tensor{\theta}{^b}\right){\tensor{p}{^j}}^2}
    -\frac{\tan_\lambda^\ast\left(\tensor{\theta}{^b}\right)}{\tan_\lambda\left(\tensor{\theta}{^a}\right)}{\tensor{p}{^{a+1}}}^2
    \right)                                                                                           \\
     & =
    \tan_\lambda\left(\tensor{\theta}{^b}\right)
    \tan_\lambda\left(\tensor{\theta}{^a}\right)
    \prod_{a\le j\le n+1}{\cos_\lambda^2\tensor{\theta}{^j}}
    \left(
    \left(\sign{\lambda}\right)
    \prod_{1\le j<a}{\cos_\lambda^2\tensor{\theta}{^j}}
    +\sum{
      \sin_\lambda^2{\tensor{\theta}{^{i}}}\prod_{i<j<a}{\cos_\lambda^2\tensor{\theta}{^j}}
    }
    -\sign{\lambda}
    \right)                                                                                           \\
     & =
    \tan_\lambda\left(\tensor{\theta}{^b}\right)
    \tan_\lambda\left(\tensor{\theta}{^a}\right)
    \prod_{a\le j\le n+1}{\cos_\lambda^2\tensor{\theta}{^j}}
    \left(
    \left(\sign{\lambda}\right)
    \prod_{1\le j<a}{\cos_\lambda^2\tensor{\theta}{^j}}
    +\sign{\lambda}\left(
    1-\prod_{1\le j<a}{\cos_\lambda^2\tensor{\theta}{^j}}
    \right)
    -\sign{\lambda}
    \right)                                                                                           \\
    \tensor{g}{_a_b}
     & =0\text{.}
  \end{align*}
  If \(a>b\), \(\tensor{g}{_a_b}=\tensor{g}{_b_a}=0\).
  If \(a=b\),
  \begin{align*}
    \tensor{g}{_a_a}
     & =
    \left(
    \lambda
    \begin{pmatrix}
        -\tan_\lambda^\ast\tensor{\theta}{^a}\tensor{p}{^j}         \\
        \frac{1}{\tan_\lambda\tensor{\theta}{^a}}\tensor{p}{^{a+1}} \\
        0                                                           \\
      \end{pmatrix}
    \right)
    \tensor{g}{}\left[\frac{\partial}{\partial\tensor{p}{^i}}\right]
    \left(
    \lambda
    \begin{pmatrix}
        -\tan_\lambda^\ast\tensor{\theta}{^a}\tensor{p}{^j}         \\
        \frac{1}{\tan_\lambda\tensor{\theta}{^a}}\tensor{p}{^{a+1}} \\
        0
      \end{pmatrix}
    \right)     \\
     & =
    \lambda^2
    \left(
    \left(\sign{\lambda}\right)\left(\tensor{p}{^1}\tan_\lambda^\ast\tensor{\theta}{^a}\right)^2
    +\sum_j{\left(\tensor{p}{^j}\tan_\lambda^\ast\tensor{\theta}{^a}\right)^2}
    +\left(\tensor{p}{^{a+1}}\cot_\lambda\tensor{\theta}{^a}\right)^2
    \right)     \\
     & =
    \sin_\lambda^2\left(\tensor{\theta}{^a}\right)
    \prod_{a<j}{\cos_\lambda^2\tensor{\theta}{^j}}
    \left(
    \left(\sign{\lambda}\right)
    \prod_{1\le j<a}{\cos_\lambda^2\tensor{\theta}{^j}}
    +\sum_{1\le i<a}{
      \sin_\lambda^2{\tensor{\theta}{^{i}}}\prod_{i<j<a}{\cos_\lambda^2\tensor{\theta}{^j}}
    }
    +\cot_\lambda^2\left(\tensor{\theta}{^a}\right)
    \right)     \\
     & =
    \sin_\lambda^2\left(\tensor{\theta}{^a}\right)
    \prod_{a<j}{\cos_\lambda^2\tensor{\theta}{^j}}
    \left(
    \left(\sign{\lambda}\right)
    \prod_{1\le j<a}{\cos_\lambda^2\tensor{\theta}{^j}}
    +\sum_{1\le i<a}{
      \sin_\lambda^2{\tensor{\theta}{^{i}}}\prod_{i<j<a}{\cos_\lambda^2\tensor{\theta}{^j}}
    }
    +\cot_\lambda^2\left(\tensor{\theta}{^a}\right)
    \right)     \\
     & =
    \sin_\lambda^2\left(\tensor{\theta}{^a}\right)
    \prod_{a<j}{\cos_\lambda^2\tensor{\theta}{^j}}
    \left(
    \sign{\lambda}
    +\cot_\lambda^2\left(\tensor{\theta}{^a}
      \right)
    \right)     \\
     & =
    \sin_\lambda^2\left(\tensor{\theta}{^a}\right)
    \prod_{a<j}{\cos_\lambda^2\tensor{\theta}{^j}}
    \left(
    \sign{\lambda}
    +\csc_\lambda^2\left(\tensor{\theta}{^a}
      -\sign{\lambda}
      \right)
    \right)     \\
     & =
    \sin_\lambda^2\left(\tensor{\theta}{^a}\right)
    \prod_{a<j}{\cos_\lambda^2\tensor{\theta}{^j}}
    \left(
    \csc_\lambda^2\left(\tensor{\theta}{^a}
      \right)
    \right)     \\
     & =
    \prod_{a<j}{\cos_\lambda^2\tensor{\theta}{^j}}
     & \qedhere
  \end{align*}
\end{proof}
\subsubsection{Curvature}
\begin{lemma}\label{M:Christoffel}
  The Christoffel symbols of the manifold
  at the point \(P\equiv\tensor{p}{}\equiv\tensor{\theta}{}\)
  is
  \[
    \tensor{\Gamma}{^a_b_c}=\begin{cases}
      -\lambda\tan_\lambda^\ast\tensor{\theta}{^c}                                                    & \text{\(a=b<c\)} \\
      -\lambda\tan_\lambda^\ast\tensor{\theta}{^b}                                                    & \text{\(a=c<b\)} \\
      +\lambda\tan_\lambda^\ast\tensor{\theta}{^a}\prod_{b<i\le a}{\cos_\lambda^2\tensor{\theta}{^i}} & \text{\(b=c<a\)} \\
      0                                                                                               & \text{otherwise} \\
    \end{cases}
  \]
\end{lemma}
\begin{proof}[Proof of \cref{M:Christoffel}]
  \begin{align*}
    \tensor{g}{_a_b_{,c}}
     & =\begin{cases}
          \frac{\partial}{\partial\tensor{\theta}{^c}}\prod_{a<i}{\cos_\lambda^2\tensor{\theta}{^i}} & \text{\(a=b\)}   \\
          \frac{\partial}{\partial\tensor{\theta}{^c}}0                                              & \text{otherwise} \\
        \end{cases}    \\
     & =\begin{cases}
          -2\lambda\tan_\lambda^\ast\tensor{\theta}{^c}\prod_{a<i}{\cos_\lambda^2\tensor{\theta}{^i}} & \text{\(a=b<c\)} \\
          0                                                                                           & \text{otherwise} \\
        \end{cases}       \\
     & =\begin{cases}
          -2\lambda\tan_\lambda^\ast\tensor{\theta}{^c}\tensor{g}{_a_a} & \text{\(a=b<c\)} \\
          0                                                             & \text{otherwise} \\
        \end{cases}                                         \\
    \tensor{g}{}
     & =\diag\left(\tensor{g}{_a_a}\right)                                                                                       \\
    {\tensor{g}{}}^{-1}
     & =\diag\left({\tensor{g}{_a_a}}^{-1}\right)                                                                                \\
    \tensor{g}{^a^b}
     & =\begin{cases}
          {\tensor{g}{_a_b}}^{-1} & \text{\(a=b\)}   \\
          0                       & \text{otherwise} \\
        \end{cases}                                                                        \\
    \tensor{\Gamma}{^a_b_c}
     & =
    \frac{1}{2}
    \sum_{i}\left(
    \tensor{g}{^a^i}
    \left(
      \tensor{g}{_i_b_{,c}}
      +\tensor{g}{_i_c_{,b}}
      -\tensor{g}{_b_c_{,i}}
      \right)
    \right)                                                                                                                      \\
     & =
    \frac{1}{2}
    \tensor{g}{^a^a}
    \left(
    \tensor{g}{_a_b_{,c}}
    +\tensor{g}{_a_c_{,b}}
    -\tensor{g}{_b_c_{,a}}
    \right)                                                                                                                      \\
     & =\begin{cases}
          \frac{1}{2}\tensor{g}{^a^a}\left(-2\lambda\tan_\lambda^\ast\tensor{\theta}{^c}\tensor{g}{_a_a}\right) & \text{\(a=b<c\)} \\
          \frac{1}{2}\tensor{g}{^a^a}\left(-2\lambda\tan_\lambda^\ast\tensor{\theta}{^b}\tensor{g}{_a_a}\right) & \text{\(a=c<b\)} \\
          \frac{1}{2}\tensor{g}{^a^a}\left(+2\lambda\tan_\lambda^\ast\tensor{\theta}{^a}\tensor{g}{_b_b}\right) & \text{\(b=c<a\)} \\
          0                                                                                                     & \text{otherwise} \\
        \end{cases} \\
     & =\begin{cases}
          -\lambda\tan_\lambda^\ast\tensor{\theta}{^c}                                          & \text{\(a=b<c\)} \\
          -\lambda\tan_\lambda^\ast\tensor{\theta}{^b}                                          & \text{\(a=c<b\)} \\
          +\lambda\tan_\lambda^\ast\tensor{\theta}{^a}\frac{\tensor{g}{_b_b}}{\tensor{g}{_a_a}} & \text{\(b=c<a\)} \\
          0                                                                                     & \text{otherwise} \\
        \end{cases}   \\
     & =\begin{cases}
          -\lambda\tan_\lambda^\ast\tensor{\theta}{^c}                                                    & \text{\(a=b<c\)} \\
          -\lambda\tan_\lambda^\ast\tensor{\theta}{^b}                                                    & \text{\(a=c<b\)} \\
          +\lambda\tan_\lambda^\ast\tensor{\theta}{^a}\prod_{b<i\le a}{\cos_\lambda^2\tensor{\theta}{^i}} & \text{\(b=c<a\)} \\
          0                                                                                               & \text{otherwise} \\
        \end{cases}\qedhere
  \end{align*}
\end{proof}
\begin{lemma}\label{M:CurvatureTensor}
  The curvature tensor of the manifold
  at the point \(P\equiv\tensor{p}{}\equiv\tensor{\theta}{}\)
  is
  \[
    \tensor{R}{^a_b_c_d}
    =
    \begin{cases}
      +\sign{\lambda}\lambda^2\tensor{g}{_b_b} & \text{\(a=c\ne b=d\)} \\
      -\sign{\lambda}\lambda^2\tensor{g}{_b_b} & \text{\(a=d\ne b=c\)} \\
      0                                        & \text{otherwise}      \\
    \end{cases}
  \]
\end{lemma}
\begin{proof}[Proof of \cref{M:CurvatureTensor}]
  \begin{align*}
    \tensor{\Gamma}{^a_b_c_{,d}}
     & =\begin{cases}
          \frac{\partial}{\partial\tensor{u}{^d}}\left[-\lambda\tan_\lambda^\ast\tensor{\theta}{^c}\right]                                                    & \text{\(a=b<c\)} \\
          \frac{\partial}{\partial\tensor{u}{^d}}\left[-\lambda\tan_\lambda^\ast\tensor{\theta}{^b}\right]                                                    & \text{\(a=c<b\)} \\
          \frac{\partial}{\partial\tensor{u}{^d}}\left[+\lambda\tan_\lambda^\ast\tensor{\theta}{^a}\prod_{b<i\le a}{\cos_\lambda^2\tensor{\theta}{^i}}\right] & \text{\(b=c<a\)} \\
          0                                                                                                                                                   & \text{otherwise} \\
        \end{cases} \\
     & =\begin{cases}
          -\sign{\lambda}\lambda^2\sec_\lambda^2\tensor{\theta}{^c}                                                                              & \text{\(a=b<c=d\)} \\
          -\sign{\lambda}\lambda^2\sec_\lambda^2\tensor{\theta}{^b}                                                                              & \text{\(a=c<b=d\)} \\
          +\lambda^2\left(1-\sign{\lambda}\tan_\lambda^2\tensor{\theta}{^a}\right)\prod_{b<i\le a}{\cos_\lambda^2\tensor{\theta}{^i}}            & \text{\(b=c<a=d\)} \\
          -2\lambda^2\tan_\lambda^\ast\tensor{\theta}{^a}\tan_\lambda^\ast\tensor{\theta}{^d}\prod_{b<i\le a}{\cos_\lambda^2\tensor{\theta}{^i}} & \text{\(b=c<d<a\)} \\
          0                                                                                                                                      & \text{otherwise}   \\
        \end{cases}                     \\
    \sum_{i}\left[\tensor{\Gamma}{^i_a_b}\tensor{\Gamma}{^c_i_d}\right]
     & =\begin{cases}
          \tensor{\Gamma}{^c_a_a}\tensor{\Gamma}{^c_c_d}                        & \text{\(a=b<c<d\)} \\
          \sum_{i>c}\left[\tensor{\Gamma}{^i_a_a}\tensor{\Gamma}{^c_i_c}\right] & \text{\(a=b<c=d\)} \\
          \tensor{\Gamma}{^d_a_a}\tensor{\Gamma}{^c_d_d}                        & \text{\(a=b<d<c\)} \\
          \tensor{\Gamma}{^a_a_b}\tensor{\Gamma}{^a_a_d}                        & \text{\(a=c<b,d\)} \\
          \tensor{\Gamma}{^a_a_b}\tensor{\Gamma}{^c_a_a}                        & \text{\(a=d<b,c\)} \\
          \tensor{\Gamma}{^b_a_b}\tensor{\Gamma}{^b_b_d}                        & \text{\(b=c<a,d\)} \\
          \tensor{\Gamma}{^b_a_b}\tensor{\Gamma}{^c_b_b}                        & \text{\(b=d<a,c\)} \\
          \tensor{\Gamma}{^a_a_b}\tensor{\Gamma}{^c_a_c}                        & \text{\(c=d<a<b\)} \\
          \sum_{i>a}\left[\tensor{\Gamma}{^i_a_a}\tensor{\Gamma}{^c_i_c}\right] & \text{\(c=d<a=b\)} \\
          \tensor{\Gamma}{^b_a_b}\tensor{\Gamma}{^c_b_c}                        & \text{\(c=d<b<a\)} \\
          0                                                                     & \text{otherwise}   \\
        \end{cases}                                                                                          \\
     & =\begin{cases}
          \left(
          +\lambda\tan_\lambda^\ast\tensor{\theta}{^c}\prod_{a<i\le c}\cos_\lambda^2\tensor{\theta}{^i}
          \right)
          \left(
          -\lambda\tan_\lambda^\ast\tensor{\theta}{^d}
          \right)
            & \text{\(a=b<c<d\)} \\
          \sum_{j>c}
          \left[
            \left(
            +\lambda\tan_\lambda^\ast\tensor{\theta}{^j}\prod_{a<i\le j}\cos_\lambda^2\tensor{\theta}{^i}
            \right)
            \left(
            -\lambda\tan_\lambda^\ast\tensor{\theta}{^j}
            \right)
            \right]
            & \text{\(a=b<c=d\)} \\
          \left(
          +\lambda\tan_\lambda^\ast\tensor{\theta}{^d}\prod_{a<i\le d}\cos_\lambda^2\tensor{\theta}{^i}
          \right)
          \left(
          +\lambda\tan_\lambda^\ast\tensor{\theta}{^c}\prod_{d<i\le c}\cos_\lambda^2\tensor{\theta}{^i}
          \right)
            & \text{\(a=b<d<c\)} \\
          \left(
          -\lambda\tan_\lambda^\ast\tensor{\theta}{^b}
          \right)
          \left(
          -\lambda\tan_\lambda^\ast\tensor{\theta}{^d}
          \right)
            & \text{\(a=c<b,d\)} \\
          \left(
          -\lambda\tan_\lambda^\ast\tensor{\theta}{^b}
          \right)
          \left(
          +\lambda\tan_\lambda^\ast\tensor{\theta}{^c}\prod_{a<i\le c}\cos_\lambda^2\tensor{\theta}{^i}
          \right)
            & \text{\(a=d<b,c\)} \\
          \left(
          -\lambda\tan_\lambda^\ast\tensor{\theta}{^a}
          \right)
          \left(
          -\lambda\tan_\lambda^\ast\tensor{\theta}{^d}
          \right)
            & \text{\(b=c<a,d\)} \\
          \left(
          -\lambda\tan_\lambda^\ast\tensor{\theta}{^a}
          \right)
          \left(
          +\lambda\tan_\lambda^\ast\tensor{\theta}{^c}\prod_{b<i\le c}\cos_\lambda^2\tensor{\theta}{^i}
          \right)
            & \text{\(b=d<a,c\)} \\
          \left(
          -\lambda\tan_\lambda^\ast\tensor{\theta}{^b}
          \right)
          \left(
          -\lambda\tan_\lambda^\ast\tensor{\theta}{^a}
          \right)
            & \text{\(c=d<a<b\)} \\
          \sum_{j>a}
          \left[
            \left(
            +\lambda\tan_\lambda^\ast\tensor{\theta}{^j}\prod_{a<i\le j}\cos_\lambda^2\tensor{\theta}{^i}
            \right)
            \left(
            -\lambda\tan_\lambda^\ast\tensor{\theta}{^j}
            \right)
            \right]
            & \text{\(c=d<a=b\)} \\
          \left(
          -\lambda\tan_\lambda^\ast\tensor{\theta}{^a}
          \right)
          \left(
          -\lambda\tan_\lambda^\ast\tensor{\theta}{^b}
          \right)
            & \text{\(c=d<b<a\)} \\
          0 & \text{otherwise}   \\
        \end{cases}                                                                                        \\
     & =\begin{cases}
          -\lambda^2\tan_\lambda^\ast\tensor{\theta}{^c}\tan_\lambda^\ast\tensor{\theta}{^d}\prod_{a<i\le c}\cos_\lambda^2\tensor{\theta}{^i}
            & \text{\(a=b<c<d\)} \\
          -\lambda^2
          \sum_{j>c}
          \left[
            \tan_\lambda^2\tensor{\theta}{^j}\prod_{a<i\le j}\cos_\lambda^2\tensor{\theta}{^i}
            \right]
            & \text{\(a=b<c=d\)} \\
          +\lambda^2\tan_\lambda^\ast\tensor{\theta}{^c}\tan_\lambda^\ast\tensor{\theta}{^d}\prod_{a<i\le c}\cos_\lambda^2\tensor{\theta}{^i}
            & \text{\(a=b<d<c\)} \\
          +\lambda^2\tan_\lambda^\ast\tensor{\theta}{^b}\tan_\lambda^\ast\tensor{\theta}{^d}
            & \text{\(a=c<b,d\)} \\
          -\lambda^2\tan_\lambda^\ast\tensor{\theta}{^b}\tan_\lambda^\ast\tensor{\theta}{^c}\prod_{a<i\le c}\cos_\lambda^2\tensor{\theta}{^i}
            & \text{\(a=d<b,c\)} \\
          +\lambda^2\tan_\lambda^\ast\tensor{\theta}{^a}\tan_\lambda^\ast\tensor{\theta}{^d}
            & \text{\(b=c<a,d\)} \\
          -\lambda^2\tan_\lambda^\ast\tensor{\theta}{^a}\tan_\lambda^\ast\tensor{\theta}{^c}\prod_{b<i\le c}\cos_\lambda^2\tensor{\theta}{^i}
            & \text{\(b=d<a,c\)} \\
          +\lambda^2\tan_\lambda^\ast\tensor{\theta}{^a}\tan_\lambda^\ast\tensor{\theta}{^b}
            & \text{\(c=d<a<b\)} \\
          -\lambda^2
          \sum_{j>a}
          \left[
            \tan_\lambda^2\tensor{\theta}{^j}\prod_{a<i\le j}\cos_\lambda^2\tensor{\theta}{^i}
            \right]
            & \text{\(c=d<a=b\)} \\
          +\lambda^2\tan_\lambda^\ast\tensor{\theta}{^a}\tan_\lambda^\ast\tensor{\theta}{^b}
            & \text{\(c=d<b<a\)} \\
          0 & \text{otherwise}   \\
        \end{cases}                                                  \\
     & =\begin{cases}
          -\lambda^2\tan_\lambda^\ast\tensor{\theta}{^c}\tan_\lambda^\ast\tensor{\theta}{^d}\prod_{a<i\le c}\cos_\lambda^2\tensor{\theta}{^i}
            & \text{\(a=b<c<d\)} \\
          -\lambda^2
          \sum_{j>c}
          \left[
            \sin_\lambda^2\tensor{\theta}{^j}\prod_{c<i<j}\cos_\lambda^2\tensor{\theta}{^i}
            \right]
          \prod_{a<i\le c}\cos_\lambda^2\tensor{\theta}{^i}
            & \text{\(a=b<c=d\)} \\
          +\lambda^2\tan_\lambda^\ast\tensor{\theta}{^c}\tan_\lambda^\ast\tensor{\theta}{^d}\prod_{a<i\le c}\cos_\lambda^2\tensor{\theta}{^i}
            & \text{\(a=b<d<c\)} \\
          +\lambda^2\tan_\lambda^\ast\tensor{\theta}{^b}\tan_\lambda^\ast\tensor{\theta}{^d}
            & \text{\(a=c<b,d\)} \\
          -\lambda^2\tan_\lambda^\ast\tensor{\theta}{^b}\tan_\lambda^\ast\tensor{\theta}{^c}\prod_{a<i\le c}\cos_\lambda^2\tensor{\theta}{^i}
            & \text{\(a=d<b,c\)} \\
          +\lambda^2\tan_\lambda^\ast\tensor{\theta}{^a}\tan_\lambda^\ast\tensor{\theta}{^d}
            & \text{\(b=c<a,d\)} \\
          -\lambda^2\tan_\lambda^\ast\tensor{\theta}{^a}\tan_\lambda^\ast\tensor{\theta}{^c}\prod_{b<i\le c}\cos_\lambda^2\tensor{\theta}{^i}
            & \text{\(b=d<a,c\)} \\
          +\lambda^2\tan_\lambda^\ast\tensor{\theta}{^a}\tan_\lambda^\ast\tensor{\theta}{^b}
            & \text{\(c=d<a<b\)} \\
          -\lambda^2
          \sum_{j>a}
          \left[
            \sin_\lambda^2\tensor{\theta}{^j}\prod_{a<i<j}\cos_\lambda^2\tensor{\theta}{^i}
            \right]
            & \text{\(c=d<a=b\)} \\
          +\lambda^2\tan_\lambda^\ast\tensor{\theta}{^a}\tan_\lambda^\ast\tensor{\theta}{^b}
            & \text{\(c=d<b<a\)} \\
          0 & \text{otherwise}   \\
        \end{cases}                                                  \\
     & =\begin{cases}
          -\lambda^2\tan_\lambda^\ast\tensor{\theta}{^c}\tan_\lambda^\ast\tensor{\theta}{^d}\prod_{a<i\le c}\cos_\lambda^2\tensor{\theta}{^i}
            & \text{\(a=b<c<d\)} \\
          -\lambda^2
          \left(
          1-\sign{\lambda}\prod_{c<i}\cos_\lambda^2\tensor{\theta}{^i}
          \right)
          \prod_{a<i\le c}\cos_\lambda^2\tensor{\theta}{^i}
            & \text{\(a=b<c=d\)} \\
          +\lambda^2\tan_\lambda^\ast\tensor{\theta}{^c}\tan_\lambda^\ast\tensor{\theta}{^d}\prod_{a<i\le c}\cos_\lambda^2\tensor{\theta}{^i}
            & \text{\(a=b<d<c\)} \\
          +\lambda^2\tan_\lambda^\ast\tensor{\theta}{^b}\tan_\lambda^\ast\tensor{\theta}{^d}
            & \text{\(a=c<b,d\)} \\
          -\lambda^2\tan_\lambda^\ast\tensor{\theta}{^b}\tan_\lambda^\ast\tensor{\theta}{^c}\prod_{a<i\le c}\cos_\lambda^2\tensor{\theta}{^i}
            & \text{\(a=d<b,c\)} \\
          +\lambda^2\tan_\lambda^\ast\tensor{\theta}{^a}\tan_\lambda^\ast\tensor{\theta}{^d}
            & \text{\(b=c<a,d\)} \\
          -\lambda^2\tan_\lambda^\ast\tensor{\theta}{^a}\tan_\lambda^\ast\tensor{\theta}{^c}\prod_{b<i\le c}\cos_\lambda^2\tensor{\theta}{^i}
            & \text{\(b=d<a,c\)} \\
          +\lambda^2\tan_\lambda^\ast\tensor{\theta}{^a}\tan_\lambda^\ast\tensor{\theta}{^b}
            & \text{\(c=d<a<b\)} \\
          -\lambda^2
          \left(
          1-\sign{\lambda}\prod_{a<i}\cos_\lambda^2\tensor{\theta}{^i}
          \right)
            & \text{\(c=d<a=b\)} \\
          +\lambda^2\tan_\lambda^\ast\tensor{\theta}{^a}\tan_\lambda^\ast\tensor{\theta}{^b}
            & \text{\(c=d<b<a\)} \\
          0 & \text{otherwise}   \\
        \end{cases}                                                  \\
     & =\begin{cases}
          -\lambda^2\tan_\lambda^\ast\tensor{\theta}{^c}\tan_\lambda^\ast\tensor{\theta}{^d}\prod_{a<i\le c}\cos_\lambda^2\tensor{\theta}{^i}
            & \text{\(a=b<c<d\)}    \\
          -\lambda^2
          \left(
          1-\sign{\lambda}\prod_{c<i}\cos_\lambda^2\tensor{\theta}{^i}
          \right)
          \prod_{a<i\le c}\cos_\lambda^2\tensor{\theta}{^i}
            & \text{\(a=b<c=d\)}    \\
          +\lambda^2\tan_\lambda^\ast\tensor{\theta}{^c}\tan_\lambda^\ast\tensor{\theta}{^d}\prod_{a<i\le c}\cos_\lambda^2\tensor{\theta}{^i}
            & \text{\(a=b<d<c\)}    \\
          +\lambda^2\tan_\lambda^\ast\tensor{\theta}{^b}\tan_\lambda^\ast\tensor{\theta}{^d}
            & \text{\(a=c<b,d\)}    \\
          -\lambda^2\tan_\lambda^\ast\tensor{\theta}{^b}\tan_\lambda^\ast\tensor{\theta}{^c}\prod_{a<i\le c}\cos_\lambda^2\tensor{\theta}{^i}
            & \text{\(a=d<b,c\)}    \\
          +\lambda^2\tan_\lambda^\ast\tensor{\theta}{^a}\tan_\lambda^\ast\tensor{\theta}{^d}
            & \text{\(b=c<a,d\)}    \\
          -\lambda^2\tan_\lambda^\ast\tensor{\theta}{^a}\tan_\lambda^\ast\tensor{\theta}{^c}\prod_{b<i\le c}\cos_\lambda^2\tensor{\theta}{^i}
            & \text{\(b=d<a,c\)}    \\
          +\lambda^2\tan_\lambda^\ast\tensor{\theta}{^a}\tan_\lambda^\ast\tensor{\theta}{^b}
            & \text{\(c=d<a\ne b\)} \\
          -\lambda^2
          \left(
          1-\sign{\lambda}\prod_{a<i}\cos_\lambda^2\tensor{\theta}{^i}
          \right)
            & \text{\(c=d<a=b\)}    \\
          0 & \text{otherwise}      \\
        \end{cases}                                                  \\
    \tensor{\Gamma}{^a_b_c_{,d}}
    +\sum_{i}\left[\tensor{\Gamma}{^i_b_c}\tensor{\Gamma}{^a_i_d}\right]
     & =\begin{cases}
          -\sign{\lambda}\lambda^2\sec_\lambda^2\tensor{\theta}{^c}                                                                              & \text{\(a=b<c=d\)} \\
          -\sign{\lambda}\lambda^2\sec_\lambda^2\tensor{\theta}{^b}                                                                              & \text{\(a=c<b=d\)} \\
          +\lambda^2\left(1-\sign{\lambda}\tan_\lambda^2\tensor{\theta}{^a}\right)\prod_{b<i\le a}{\cos_\lambda^2\tensor{\theta}{^i}}            & \text{\(b=c<a=d\)} \\
          -2\lambda^2\tan_\lambda^\ast\tensor{\theta}{^a}\tan_\lambda^\ast\tensor{\theta}{^d}\prod_{b<i\le a}{\cos_\lambda^2\tensor{\theta}{^i}} & \text{\(b=c<d<a\)} \\
          0                                                                                                                                      & \text{otherwise}   \\
        \end{cases}                     \\
     & +\begin{cases}
          +\lambda^2\tan_\lambda^\ast\tensor{\theta}{^c}\tan_\lambda^\ast\tensor{\theta}{^d}
            & \text{\(a=b<c,d\)}    \\
          +\lambda^2\tan_\lambda^\ast\tensor{\theta}{^b}\tan_\lambda^\ast\tensor{\theta}{^d}
            & \text{\(a=c<b,d\)}    \\
          +\lambda^2\tan_\lambda^\ast\tensor{\theta}{^b}\tan_\lambda^\ast\tensor{\theta}{^c}
            & \text{\(a=d<b\ne c\)} \\
          -\lambda^2
          \left(
          1-\sign{\lambda}\prod_{b<i}\cos_\lambda^2\tensor{\theta}{^i}
          \right)
            & \text{\(a=d<b=c\)}    \\
          -\lambda^2\tan_\lambda^\ast\tensor{\theta}{^a}\tan_\lambda^\ast\tensor{\theta}{^d}\prod_{b<i\le a}\cos_\lambda^2\tensor{\theta}{^i}
            & \text{\(b=c<a<d\)}    \\
          -\lambda^2
          \left(
          1-\sign{\lambda}\prod_{a<i}\cos_\lambda^2\tensor{\theta}{^i}
          \right)
          \prod_{b<i\le a}\cos_\lambda^2\tensor{\theta}{^i}
            & \text{\(b=c<a=d\)}    \\
          +\lambda^2\tan_\lambda^\ast\tensor{\theta}{^a}\tan_\lambda^\ast\tensor{\theta}{^d}\prod_{b<i\le a}\cos_\lambda^2\tensor{\theta}{^i}
            & \text{\(b=c<d<a\)}    \\
          -\lambda^2\tan_\lambda^\ast\tensor{\theta}{^c}\tan_\lambda^\ast\tensor{\theta}{^a}\prod_{b<i\le a}\cos_\lambda^2\tensor{\theta}{^i}
            & \text{\(b=d<a,c\)}    \\
          -\lambda^2\tan_\lambda^\ast\tensor{\theta}{^b}\tan_\lambda^\ast\tensor{\theta}{^a}\prod_{c<i\le a}\cos_\lambda^2\tensor{\theta}{^i}
            & \text{\(c=d<a,b\)}    \\
          0 & \text{otherwise}      \\
        \end{cases}                                                  \\
     & =\begin{cases}
          +\lambda^2\tan_\lambda^\ast\tensor{\theta}{^c}\tan_\lambda^\ast\tensor{\theta}{^d}
            & \text{\(a=b<c\ne d\)} \\
          -\sign{\lambda}\lambda^2\sec_\lambda^2\tensor{\theta}{^c}
          +\lambda^2\tan_\lambda^2\tensor{\theta}{^c}
            & \text{\(a=b<c=d\)}    \\
          +\lambda^2\tan_\lambda^\ast\tensor{\theta}{^b}\tan_\lambda^\ast\tensor{\theta}{^d}
            & \text{\(a=c<b\ne d\)} \\
          -\sign{\lambda}\lambda^2\sec^2_\lambda\tensor{\theta}{^b}
          +\lambda^2\tan_\lambda^2\tensor{\theta}{^b}
            & \text{\(a=c<b=d\)}    \\
          +\lambda^2\tan_\lambda^\ast\tensor{\theta}{^b}\tan_\lambda^\ast\tensor{\theta}{^c}
            & \text{\(a=d<b\ne c\)} \\
          -\lambda^2
          \left(
          1-\sign{\lambda}\prod_{b<i}\cos_\lambda^2\tensor{\theta}{^i}
          \right)
            & \text{\(a=d<b=c\)}    \\
          -\lambda^2\tan_\lambda^\ast\tensor{\theta}{^a}\tan_\lambda^\ast\tensor{\theta}{^d}\prod_{b<i\le a}\cos_\lambda^2\tensor{\theta}{^i}
            & \text{\(b=c<a<d\)}    \\
          +\lambda^2\left(1-\sign{\lambda}\tan_\lambda^2\tensor{\theta}{^a}\right)\prod_{b<i\le a}{\cos_\lambda^2\tensor{\theta}{^i}}
          -\lambda^2
          \left(
          1-\sign{\lambda}\prod_{a<i}\cos_\lambda^2\tensor{\theta}{^i}
          \right)
          \prod_{b<i\le a}\cos_\lambda^2\tensor{\theta}{^i}
            & \text{\(b=c<a=d\)}    \\
          -2\lambda^2\tan_\lambda^\ast\tensor{\theta}{^a}\tan_\lambda^\ast\tensor{\theta}{^d}\prod_{b<i\le a}{\cos_\lambda^2\tensor{\theta}{^i}}
          +\lambda^2\tan_\lambda^\ast\tensor{\theta}{^a}\tan_\lambda^\ast\tensor{\theta}{^d}\prod_{b<i\le a}\cos_\lambda^2\tensor{\theta}{^i}
            & \text{\(b=c<d<a\)}    \\
          -\lambda^2\tan_\lambda^\ast\tensor{\theta}{^c}\tan_\lambda^\ast\tensor{\theta}{^a}\prod_{b<i\le a}\cos_\lambda^2\tensor{\theta}{^i}
            & \text{\(b=d<a,c\)}    \\
          -\lambda^2\tan_\lambda^\ast\tensor{\theta}{^b}\tan_\lambda^\ast\tensor{\theta}{^a}\prod_{c<i\le a}\cos_\lambda^2\tensor{\theta}{^i}
            & \text{\(c=d<a,b\)}    \\
          0 & \text{otherwise}      \\
        \end{cases}                                           \\
     & =\begin{cases}
          +\lambda^2\tan_\lambda^\ast\tensor{\theta}{^c}\tan_\lambda^\ast\tensor{\theta}{^d}
            & \text{\(a=b<c\ne d\)} \\
          -\sign{\lambda}\lambda^2
            & \text{\(a=b<c=d\)}    \\
          +\lambda^2\tan_\lambda^\ast\tensor{\theta}{^b}\tan_\lambda^\ast\tensor{\theta}{^d}
            & \text{\(a=c<b\ne d\)} \\
          -\sign{\lambda}\lambda^2
            & \text{\(a=c<b=d\)}    \\
          +\lambda^2\tan_\lambda^\ast\tensor{\theta}{^b}\tan_\lambda^\ast\tensor{\theta}{^c}
            & \text{\(a=d<b\ne c\)} \\
          -\lambda^2
          \left(
          1-\sign{\lambda}\prod_{b<i}\cos_\lambda^2\tensor{\theta}{^i}
          \right)
            & \text{\(a=d<b=c\)}    \\
          -\lambda^2\tan_\lambda^\ast\tensor{\theta}{^a}\tan_\lambda^\ast\tensor{\theta}{^d}\prod_{b<i\le a}\cos_\lambda^2\tensor{\theta}{^i}
            & \text{\(b=c<a<d\)}    \\
          +\sign{\lambda}\lambda^2
          \left(
          -\tan_\lambda^2\tensor{\theta}{^a}
          +\prod_{a<i}\cos_\lambda^2\tensor{\theta}{^i}
          \right)
          \prod_{b<i\le a}{\cos_\lambda^2\tensor{\theta}{^i}}
            & \text{\(b=c<a=d\)}    \\
          -\lambda^2\tan_\lambda^\ast\tensor{\theta}{^a}\tan_\lambda^\ast\tensor{\theta}{^d}\prod_{b<i\le a}{\cos_\lambda^2\tensor{\theta}{^i}}
            & \text{\(b=c<d<a\)}    \\
          -\lambda^2\tan_\lambda^\ast\tensor{\theta}{^c}\tan_\lambda^\ast\tensor{\theta}{^a}\prod_{b<i\le a}\cos_\lambda^2\tensor{\theta}{^i}
            & \text{\(b=d<a,c\)}    \\
          -\lambda^2\tan_\lambda^\ast\tensor{\theta}{^b}\tan_\lambda^\ast\tensor{\theta}{^a}\prod_{c<i\le a}\cos_\lambda^2\tensor{\theta}{^i}
            & \text{\(c=d<a,b\)}    \\
          0 & \text{otherwise}      \\
        \end{cases}                                            \\
    \tensor{R}{^a_b_c_d}
     & =
    \tensor{\Gamma}{^a_b_d_{,c}}
    -\tensor{\Gamma}{^a_b_c_{,d}}
    +\sum_{i}\left[\tensor{\Gamma}{^i_b_d}\tensor{\Gamma}{^a_i_c}-\tensor{\Gamma}{^i_b_c}\tensor{\Gamma}{^a_i_d}\right]
    \\
     & =
    -\left(
    \tensor{\Gamma}{^a_b_c_{,d}}
    +\sum_{i}\left[\tensor{\Gamma}{^i_b_c}\tensor{\Gamma}{^a_i_d}\right]
    \right)
    +\left(
    \tensor{\Gamma}{^a_b_d_{,c}}
    +\sum_{i}\left[\tensor{\Gamma}{^i_b_d}\tensor{\Gamma}{^a_i_c}\right]
    \right)                                                                                                                                                                                 \\
     & =-
    \begin{cases}
      +\lambda^2\tan_\lambda^\ast\tensor{\theta}{^c}\tan_\lambda^\ast\tensor{\theta}{^d}
        & \text{\(a=b<c\ne d\)} \\
      -\sign{\lambda}\lambda^2
        & \text{\(a=b<c=d\)}    \\
      +\lambda^2\tan_\lambda^\ast\tensor{\theta}{^b}\tan_\lambda^\ast\tensor{\theta}{^d}
        & \text{\(a=c<b\ne d\)} \\
      -\sign{\lambda}\lambda^2
        & \text{\(a=c<b=d\)}    \\
      +\lambda^2\tan_\lambda^\ast\tensor{\theta}{^b}\tan_\lambda^\ast\tensor{\theta}{^c}
        & \text{\(a=d<b\ne c\)} \\
      -\lambda^2
      \left(
      1
      -\sign{\lambda}\prod_{b<i}\cos_\lambda^2\tensor{\theta}{^i}
      \right)
        & \text{\(a=d<b=c\)}    \\
      -\lambda^2\tan_\lambda^\ast\tensor{\theta}{^a}\tan_\lambda^\ast\tensor{\theta}{^d}\prod_{b<i\le a}\cos_\lambda^2\tensor{\theta}{^i}
        & \text{\(b=c<a<d\)}    \\
      +\sign{\lambda}\lambda^2
      \left(
      -\tan_\lambda^2\tensor{\theta}{^a}
      +\prod_{a<i}\cos_\lambda^2\tensor{\theta}{^i}
      \right)
      \prod_{b<i\le a}\cos_\lambda^2\tensor{\theta}{^i}
        & \text{\(b=c<a=d\)}    \\
      -\lambda^2\tan_\lambda^\ast\tensor{\theta}{^a}\tan_\lambda^\ast\tensor{\theta}{^d}\prod_{b<i\le a}{\cos_\lambda^2\tensor{\theta}{^i}}
        & \text{\(b=c<d<a\)}    \\
      -\lambda^2\tan_\lambda^\ast\tensor{\theta}{^a}\tan_\lambda^\ast\tensor{\theta}{^c}\prod_{b<i\le a}\cos_\lambda^2\tensor{\theta}{^i}
        & \text{\(b=d<a,c\)}    \\
      -\lambda^2\tan_\lambda^\ast\tensor{\theta}{^a}\tan_\lambda^\ast\tensor{\theta}{^b}\prod_{c<i\le a}\cos_\lambda^2\tensor{\theta}{^i}
        & \text{\(c=d<a,b\)}    \\
      0 & \text{otherwise}      \\
    \end{cases}                                                \\
     & +\begin{cases}
          +\lambda^2\tan_\lambda^\ast\tensor{\theta}{^c}\tan_\lambda^\ast\tensor{\theta}{^d}
            & \text{\(a=b<c\ne d\)} \\
          -\sign{\lambda}\lambda^2
            & \text{\(a=b<c=d\)}    \\
          +\lambda^2\tan_\lambda^\ast\tensor{\theta}{^b}\tan_\lambda^\ast\tensor{\theta}{^d}
            & \text{\(a=c<b\ne d\)} \\
          -\lambda^2
          \left(
          1
          -\sign{\lambda}\prod_{b<i}\cos_\lambda^2\tensor{\theta}{^i}
          \right)
            & \text{\(a=c<b=d\)}    \\
          +\lambda^2\tan_\lambda^\ast\tensor{\theta}{^b}\tan_\lambda^\ast\tensor{\theta}{^c}
            & \text{\(a=d<b\ne c\)} \\
          -\sign{\lambda}\lambda^2
            & \text{\(a=d<b=c\)}    \\
          -\lambda^2\tan_\lambda^\ast\tensor{\theta}{^d}\tan_\lambda^\ast\tensor{\theta}{^a}\prod_{b<i\le a}\cos_\lambda^2\tensor{\theta}{^i}
            & \text{\(b=c<a,d\)}    \\
          -\lambda^2\tan_\lambda^\ast\tensor{\theta}{^a}\tan_\lambda^\ast\tensor{\theta}{^c}\prod_{b<i\le a}\cos_\lambda^2\tensor{\theta}{^i}
            & \text{\(b=d<a<c\)}    \\
          +\sign{\lambda}\lambda^2
          \left(
          -\tan_\lambda^2\tensor{\theta}{^a}
          +\prod_{a<i}\cos_\lambda^2\tensor{\theta}{^i}
          \right)
          \prod_{b<i\le a}\cos_\lambda^2\tensor{\theta}{^i}
            & \text{\(b=d<a=c\)}    \\
          -\lambda^2\tan_\lambda^\ast\tensor{\theta}{^a}\tan_\lambda^\ast\tensor{\theta}{^c}\prod_{b<i\le a}{\cos_\lambda^2\tensor{\theta}{^i}}
            & \text{\(b=d<c<a\)}    \\
          -\lambda^2\tan_\lambda^\ast\tensor{\theta}{^b}\tan_\lambda^\ast\tensor{\theta}{^a}\prod_{c<i\le a}\cos_\lambda^2\tensor{\theta}{^i}
            & \text{\(c=d<a,b\)}    \\
          0 & \text{otherwise}      \\
        \end{cases}                                            \\
     & =\begin{cases}
          +\sign{\lambda}\lambda^2
          \prod_{b<i}\cos_\lambda^2\tensor{\theta}{^i}
            & \text{\(a=c<b=d\)} \\
          -\sign{\lambda}\lambda^2
          \prod_{b<i}\cos_\lambda^2\tensor{\theta}{^i}
            & \text{\(a=d<b=c\)} \\
          -\sign{\lambda}\lambda^2
          \prod_{b<i}\cos_\lambda^2\tensor{\theta}{^i}
            & \text{\(b=c<a=d\)} \\
          +\sign{\lambda}\lambda^2
          \prod_{b<i}\cos_\lambda^2\tensor{\theta}{^i}
            & \text{\(b=d<a=c\)} \\
          0 & \text{otherwise}   \\
        \end{cases}                                                                                                                                         \\
     & =\begin{cases}
          +\sign{\lambda}\lambda^2\tensor{g}{_b_b}
            & \text{\(a=c\ne b=d\)} \\
          -\sign{\lambda}\lambda^2\tensor{g}{_b_b}
            & \text{\(a=d\ne b=c\)} \\
          0 & \text{otherwise}      \\
        \end{cases}\qedhere
  \end{align*}
\end{proof}
\begin{lemma}\label{M:SectionalCurvature}
  The sectional curvature of the manifold
  at the point \(P\equiv\tensor{p}{}\equiv\tensor{\theta}{}\)
  along the tangent vector \(\tensor{u}{}\) and \(\tensor{v}{}\)
  is
  \[
    K\left(\tensor{u}{},\tensor{v}{}\right)=\sign{\lambda}\lambda^2
  \]
\end{lemma}
\begin{proof}[Proof of \cref{M:SectionalCurvature}]
  \begin{align*}
    K\left(\tensor{u}{},\tensor{v}{}\right)
     & =
    \frac{
      \left\langle{R\left(\tensor{u}{},\tensor{v}{}\right)\tensor{v}{}},{\tensor{u}{}}\right\rangle
    }{
      \left\langle{\tensor{u}{}},{\tensor{u}{}}\right\rangle
      \left\langle{\tensor{v}{}},{\tensor{v}{}}\right\rangle
      -\left\langle{\tensor{u}{}},{\tensor{v}{}}\right\rangle^2
    }    \\
     & =
    \frac{
      \left\langle{
        \contr{\left(\contr^2{\left(\tensor{R}{}\otimes\tensor{v}{}\otimes\tensor{u}{}\right)}\otimes\tensor{v}{}\right)}
      },{\tensor{u}{}}\right\rangle
    }{
      \left\langle{\tensor{u}{}},{\tensor{u}{}}\right\rangle
      \left\langle{\tensor{v}{}},{\tensor{v}{}}\right\rangle
      -\left\langle{\tensor{u}{}},{\tensor{v}{}}\right\rangle^2
    }    \\
     & =
    \frac{
    \contr^2{\left(\tensor{g}{}\otimes\tensor{u}{}\otimes\contr^3\left(\tensor{R}{}\otimes\tensor{v}{}\otimes\tensor{u}{}\otimes\tensor{v}{}\right)\right)}
    }{
    \contr^2{\left(\tensor{g}{}\otimes\tensor{u}{}\otimes\tensor{u}{}\right)}
    \contr^2{\left(\tensor{g}{}\otimes\tensor{v}{}\otimes\tensor{v}{}\right)}
    -\contr^2{\left(\tensor{g}{}\otimes\tensor{u}{}\otimes\tensor{v}{}\right)}^2
    }    \\
     & =
    \frac{
      \sum_{i,j,a,b,c}\left[\tensor{g}{_i_j}\tensor{u}{^j}\tensor{R}{^i_c_a_b}\tensor{v}{^b}\tensor{u}{^a}\tensor{v}{^c}\right]
    }{
      \sum_{i,j}\left[\tensor{g}{_i_j}\tensor{u}{^j}\tensor{u}{^i}\right]
      \sum_{i,j}\left[\tensor{g}{_i_j}\tensor{v}{^j}\tensor{v}{^i}\right]
      -\left(\sum_{i,j}\left[\tensor{g}{_i_j}\tensor{v}{^j}\tensor{u}{^i}\right]\right)^2
    }    \\
     & =
    \frac{
      \sum_{i,a,b,c}\left[\tensor{g}{_i_i}\tensor{u}{^i}\tensor{R}{^i_c_a_b}\tensor{v}{^b}\tensor{u}{^a}\tensor{v}{^c}\right]
    }{
      \sum_{i}\left[\tensor{g}{_i_i}\tensor{u}{^i}\tensor{u}{^i}\right]
      \sum_{i}\left[\tensor{g}{_i_i}\tensor{v}{^i}\tensor{v}{^i}\right]
      -\left(\sum_{i}\left[\tensor{g}{_i_i}\tensor{v}{^i}\tensor{u}{^i}\right]\right)^2
    }    \\
     & =
    \frac{
      \sum_{i,a,b,c}\left[\tensor{g}{_i_i}\tensor{u}{^i}\tensor{R}{^i_c_a_b}\tensor{v}{^b}\tensor{u}{^a}\tensor{v}{^c}\right]
    }{
      \sum_{i}\left[\tensor{g}{_i_i}\tensor{u}{^i}\tensor{u}{^i}\right]
      \sum_{i}\left[\tensor{g}{_i_i}\tensor{v}{^i}\tensor{v}{^i}\right]
      -\left(\sum_{i}\left[\tensor{g}{_i_i}\tensor{v}{^i}\tensor{u}{^i}\right]\right)^2
    }    \\
     & =
    \frac{
      \sum_{i\ne j}\left[
        \tensor{g}{_i_i}
        \tensor{u}{^i}
        \tensor{R}{^i_j_i_j}
        \tensor{v}{^j}
        \tensor{u}{^i}
        \tensor{v}{^j}
        -
        \tensor{g}{_i_i}
        \tensor{u}{^i}
        \tensor{R}{^i_j_j_i}
        \tensor{v}{^i}
        \tensor{u}{^j}
        \tensor{v}{^j}
        \right]
    }{
      \sum_{i,j}\left[
        \tensor{g}{_i_i}\tensor{u}{^i}\tensor{u}{^i}
        \tensor{g}{_j_j}\tensor{u}{^j}\tensor{u}{^j}
        -
        \tensor{g}{_i_i}\tensor{v}{^i}\tensor{u}{^i}
        \tensor{g}{_j_j}\tensor{v}{^j}\tensor{u}{^j}
        \right]
    }    \\
     & =
    \frac{
      \sum_{i\ne j}\left[
        +\sign{\lambda}\lambda^2
        \tensor{g}{_i_i}
        \tensor{u}{^i}
        \tensor{g}{_j_j}
        \tensor{v}{^j}
        \tensor{u}{^i}
        \tensor{v}{^j}
        +\sign{\lambda}\lambda^2
        \tensor{g}{_i_i}
        \tensor{u}{^i}
        \tensor{g}{_j_j}
        \tensor{v}{^i}
        \tensor{u}{^j}
        \tensor{v}{^j}
        \right]
    }{
      \sum_{i\ne j}\left[
        \tensor{g}{_i_i}\tensor{u}{^i}\tensor{u}{^i}
        \tensor{g}{_j_j}\tensor{u}{^j}\tensor{u}{^j}
        -
        \tensor{g}{_i_i}\tensor{v}{^i}\tensor{u}{^i}
        \tensor{g}{_j_j}\tensor{v}{^j}\tensor{u}{^j}
        \right]
      +
      \sum_{i}\left[
        \tensor{g}{_i_i}\tensor{u}{^i}\tensor{u}{^i}
        \tensor{g}{_i_i}\tensor{u}{^i}\tensor{u}{^i}
        -
        \tensor{g}{_i_i}\tensor{v}{^i}\tensor{u}{^i}
        \tensor{g}{_i_i}\tensor{v}{^i}\tensor{u}{^i}
        \right]
    }    \\
     & =
    \sign{\lambda}\lambda^2
    \frac{
      \sum_{i\ne j}\left[
        \tensor{g}{_i_i}
        \tensor{u}{^i}
        \tensor{u}{^i}
        \tensor{g}{_j_j}
        \tensor{v}{^j}
        \tensor{v}{^j}
        +
        \tensor{g}{_i_i}
        \tensor{g}{_j_j}
        \tensor{v}{^i}
        \tensor{u}{^i}
        \tensor{u}{^j}
        \tensor{v}{^j}
        \right]
    }{
      \sum_{i\ne j}\left[
        \tensor{g}{_i_i}\tensor{u}{^i}\tensor{u}{^i}
        \tensor{g}{_j_j}\tensor{u}{^j}\tensor{u}{^j}
        -
        \tensor{g}{_i_i}\tensor{v}{^i}\tensor{u}{^i}
        \tensor{g}{_j_j}\tensor{v}{^j}\tensor{u}{^j}
        \right]
    }    \\
     & =
    \sign{\lambda}\lambda^2 \qedhere
  \end{align*}
\end{proof}
\begin{remark}
  It can be seen that \(\operatorname{sec}\left(p\right)=\kappa=\sign{\lambda}\lambda^2\).
  Hence, when provided \(\kappa\), \(\lambda\) can be determined
  which imply that \(g\) is a valid inner product for the model.
\end{remark}
\end{document}